theories/Infra/AutoIndTac.v
@@ -1,5 +1,5 @@
-Require Import Smpl List.
-Require Export LengthEq.
+Require Import List.
+Require Export Smpl LvcPlugin LengthEq MoreInversion.
 
 Set Implicit Arguments.
 
@@ -57,8 +57,6 @@ Ltac is_ftype H :=
 
 Class DoNotRemember (T:Type) := DNR { Q:Type }.
 
-Declare ML Module "lvc_plugin".
-
 Ltac remember_arguments E :=
   let tac t x := ( try (is_param t 0; fail 1);
                   try (is_var x; fail 1);
@@ -100,11 +98,6 @@ Ltac clear_dup :=
     end
   end.
 
-Ltac clear_dup_fast :=
-  match goal with
-  | [ H : ?X, H' : ?X |- _ ] => first [clear H' || clear H]
-  end.
-
 Ltac clear_if_dup H :=
   match type of H with
     | ?X =>
@@ -117,48 +110,6 @@ Ltac clear_if_dup H :=
       end
   end.
 
-Ltac inv_eqs :=
-  repeat (match goal with
-              | [ H : @eq _ ?x ?x |- _ ] => clear H
-              | [ H : @eq _ ?x ?y |- _ ] => progress (inversion H; subst; try clear_dup)
-            end).
-
-(* this is a standard tactic *)
-
-
-Smpl Create inv_trivial.
-
-Ltac inv_trivial_base :=
-  match goal with
-  | [ H : @eq _ ?x ?x |- _ ] => clear H
-  | [ H : @eq _ ?x ?y |- _ ] => first [ is_var x; subst x | is_var y; subst y ]
-  | [ H : true = false |- _ ] => exfalso; inversion H
-  | [ H : false = true |- _ ] => exfalso; inversion H
-  | [ H : ?A = ?B |- _ ] => first [ is_constructor_app A;
-                                  match B with
-                                  | (if _ then _ else _) => fail 1
-                                  | _ => inversion H; subst
-                                  end
-                                | is_constructor_app B;
-                                  match A with
-                                  | (if _ then _ else _) => fail 1
-                                  | _ => inversion H; subst
-                                  end
-                                ]
-(*  | [ H : nil = _ :: _ |- _ ] => exfalso; discriminate H
-  | [ H : _ :: _ = _ :: _ |- _ ] => inversion H; subst *)
-  | [ H : ?n <= 0 |- _ ] => is_var n; inversion H; subst; clear H
-  | [ H : @eq _ (Some ?x) (Some ?y) |- _ ]
-    => let H' := fresh "H" in assert (H':x = y) by congruence; clear H;
-                            first [ is_var x; subst x; clear H'
-                                  | is_var y; subst y; clear H'
-                                  | rename H' into H ]
-  end.
-
-Smpl Add inv_trivial_base : inv_trivial.
-
-Ltac clear_trivial_eqs :=
-  repeat (smpl inv_trivial; repeat clear_dup_fast).
 
 Ltac inductify H :=
   match type of H with
