theories/Infra/Len.v
@@ -1,0 +1,7 @@
+Require Import Smpl.
+
+Create HintDb len discriminated.
+
+Smpl Create len.
+Ltac len_simpl := smpl len; repeat (smpl len).
+Hint Extern 0 => len_simpl : len.
