theories/Infra/MoreInversion.v
@@ -1,0 +1,84 @@
+Require Import Smpl LvcPlugin.
+
+Set Implicit Arguments.
+
+Set Regular Subst Tactic.
+
+Ltac clear_dup_fast :=
+  match goal with
+  | [ H : ?X, H' : ?X |- _ ] => first [clear H' || clear H]
+  end.
+
+Ltac inv_eqs :=
+  repeat (match goal with
+              | [ H : @eq _ ?x ?x |- _ ] => clear H
+              | [ H : @eq _ ?x ?y |- _ ] => progress (inversion H; subst; try clear_dup_fast)
+            end).
+
+
+Smpl Create inv_trivial.
+
+Ltac inv_trivial_base :=
+  match goal with
+  | [ H : @eq _ ?x ?x |- _ ] => clear H
+  | [ H : @eq _ ?x ?y |- _ ] => first [ is_var x; subst x | is_var y; subst y ]
+  | [ H : true = false |- _ ] => exfalso; inversion H
+  | [ H : false = true |- _ ] => exfalso; inversion H
+  | [ H : ?A = ?B |- _ ] => first [ is_constructor_app A;
+                                  match B with
+                                  | (if _ then _ else _) => fail 1
+                                  | _ => inversion H; subst
+                                  end
+                                | is_constructor_app B;
+                                  match A with
+                                  | (if _ then _ else _) => fail 1
+                                  | _ => inversion H; subst
+                                  end
+                                ]
+(*  | [ H : nil = _ :: _ |- _ ] => exfalso; discriminate H
+  | [ H : _ :: _ = _ :: _ |- _ ] => inversion H; subst *)
+  | [ H : ?n <= 0 |- _ ] => is_var n; inversion H; subst; clear H
+  | [ H : @eq _ (Some ?x) (Some ?y) |- _ ]
+    => let H' := fresh "H" in assert (H':x = y) by congruence; clear H;
+                            first [ is_var x; subst x; clear H'
+                                  | is_var y; subst y; clear H'
+                                  | rename H' into H ]
+  end.
+
+Smpl Add inv_trivial_base : inv_trivial.
+
+Ltac clear_trivial_eqs :=
+  repeat (smpl inv_trivial; repeat clear_dup_fast).
+
+Tactic Notation "inv" hyp(A) := inversion A; subst.
+Tactic Notation "invc" hyp(A) := inversion A; subst; (try clear A).
+Tactic Notation "invs" hyp(A) := inversion A; subst; clear_trivial_eqs.
+Tactic Notation "invcs" hyp(A) := inversion A; subst; (try clear A); clear_trivial_eqs.
+
+Ltac invt ty :=
+  match goal with
+      | h: ty |- _ => inv h
+      | h: ty _ |- _ => inv h
+      | h: ty _ _ |- _ => inv h
+      | h: ty _ _ _ |- _ => inv h
+      | h: ty _ _ _ _ |- _ => inv h
+      | h: ty _ _ _ _ _ |- _ => inv h
+      | h: ty _ _ _ _ _ _ |- _ => inv h
+      | h: ty _ _ _ _ _ _ _ |- _ => inv h
+      | h: ty _ _ _ _ _ _ _ _ |- _ => inv h
+      | h: ty _ _ _ _ _ _ _ _ _ |- _ => inv h
+  end.
+
+Ltac invts ty :=
+  match goal with
+      | h: ty |- _ => invs h
+      | h: ty _ |- _ => invs h
+      | h: ty _ _ |- _ => invs h
+      | h: ty _ _ _ |- _ => invs h
+      | h: ty _ _ _ _ |- _ => invs h
+      | h: ty _ _ _ _ _ |- _ => invs h
+      | h: ty _ _ _ _ _ _ |- _ => invs h
+      | h: ty _ _ _ _ _ _ _ |- _ => invs h
+      | h: ty _ _ _ _ _ _ _ _ |- _ => invs h
+      | h: ty _ _ _ _ _ _ _ _ _ |- _ => invs h
+  end.
