theories/Infra/Option.v
@@ -1,4 +1,4 @@
-Require Import Util List Coq.Classes.Equivalence Containers.OrderedTypeEx.
+Require Import List Coq.Classes.Equivalence Containers.OrderedTypeEx MoreInversion.
 
 (** Cast option in the framework of Monad. The code in this file is taken from CompCert. *)
 
