theories/Infra/SafeFirst.v
@@ -1,0 +1,74 @@
+Require Import Util.
+
+Set Implicit Arguments.
+
+Section SafeFirst.
+
+  Hypothesis Q : nat -> Prop.
+  Inductive safe : nat -> Prop :=
+  | safe_here n : Q n -> safe n
+  | safe_after n : safe (S n) -> safe n.
+
+  Lemma safe_antitone m n
+  : safe n
+    -> m < n
+    -> safe m.
+  Proof.
+    intros. general induction H0; eauto using safe.
+  Qed.
+
+  Lemma exists_is_safe
+  : (exists x, Q x) -> exists n, safe n.
+  Proof.
+    intros. destruct H; eexists; eauto using safe.
+  Qed.
+
+  Hypothesis comp  : forall n, Computable (Q n).
+
+  Lemma safe_upward n
+  : safe n -> ~ Q n -> safe (S n).
+  Proof.
+    intros; destruct H.
+    - destruct (H0 H).
+    - eapply H.
+  Defined.
+
+  Fixpoint safe_first n (s:safe n) : nat.
+  refine (if [ Q n ] then n else safe_first (S n) _).
+  destruct s; eauto. destruct (n0 H).
+  Defined.
+
+  Hypothesis P : nat -> Prop.
+  Hypothesis I : nat -> Prop.
+  Hypothesis PQ : forall n, P n -> Q n.
+  Hypothesis Step : forall n, I n -> ~ Q n -> I (S n).
+  Hypothesis Final : forall n , I n -> Q n -> P n.
+
+  Fixpoint safe_first_spec n s
+    : I n -> P (@safe_first n s).
+  Proof.
+    unfold safe_first.
+    destruct s.
+    - simpl. destruct (decision_procedure (Q n)); eauto.
+    - cases; eauto.
+  Qed.
+
+End SafeFirst.
+
+Fixpoint safe_first_ext P Q n
+      (PC:forall n, Computable (P n))
+      (QC:forall n, Computable (Q n))
+      (PS:safe P n)
+      (QS:safe Q n)
+      (EXT:(forall x, P x <-> Q x)) {struct PS}
+: safe_first PC PS = safe_first QC QS.
+Proof.
+  destruct PS; destruct QS; simpl; repeat cases; eauto;
+  exfalso; firstorder.
+Qed.
+
+Lemma safe_impl (P Q: nat -> Prop) n
+: safe P n -> (forall x, P x -> Q x) -> safe Q n.
+Proof.
+  intros. general induction H; eauto using safe.
+Qed.
